Prove wp_State__objListLocked

src/proof/kubernetes_model/list.v
@@ -1,4 +1,5 @@
 From New.proof Require Import prelude empty_ffi.
+From New.proof.map Require Import for_range.
 From New.proof.kubernetes_model Require Export inv common.
 
 Section proof.
@@ -14,6 +15,252 @@ Proof.
   induction 1 as [|obj objs [pod ->] _ [pods ->]].
   - exists []. done.
   - exists (pod :: pods). done.
+Qed.
+
+Definition processed_map `{Countable K} {A}
+    (keys : list K) (i : Z) (m : gmap K A) : gmap K A :=
+  filter (λ '(k, _), k ∈ list_to_set (C:=gset K) (take (Z.to_nat i) keys)) m.
+
+Lemma current_key_not_in_take `{EqDecision A} `{Countable A} (keys : list A) i key :
+  NoDup keys →
+  keys !! Z.to_nat i = Some key →
+  (0 ≤ i)%Z →
+  key ∉ list_to_set (C:=gset A) (take (Z.to_nat i) keys).
+Proof.
+  intros Hnodup Hlookup Hi_nonneg Hin.
+  rewrite elem_of_list_to_set in Hin.
+  apply list_elem_of_lookup_1 in Hin as [j Htake_lookup].
+  apply lookup_take_Some in Htake_lookup as [Hlookup_j Hj].
+  pose proof (NoDup_lookup _ _ _ _ Hnodup Hlookup_j Hlookup) as ->.
+  lia.
+Qed.
+
+Lemma processed_map_empty `{Countable K} {A} (keys : list K) (m : gmap K A) :
+  processed_map keys 0 m = ∅.
+Proof.
+  apply map_eq. intros key.
+  rewrite /processed_map map_lookup_filter lookup_empty take_0.
+  destruct (m !! key); simpl; [|done].
+  destruct (decide (key ∈ list_to_set (C:=gset K) [])); [|done].
+  rewrite elem_of_list_to_set elem_of_nil in e. done.
+Qed.
+
+Lemma processed_map_lookup_not_current `{Countable K} {A}
+    (keys : list K) i key (m : gmap K A) :
+  NoDup keys →
+  keys !! Z.to_nat i = Some key →
+  (0 ≤ i)%Z →
+  processed_map keys i m !! key = None.
+Proof.
+  intros Hnodup Hlookup Hi_nonneg.
+  rewrite /processed_map. apply map_lookup_filter_None_2. right.
+  intros x Hx Hin. simpl in Hin.
+  exact ((current_key_not_in_take keys i key Hnodup Hlookup Hi_nonneg) Hin).
+Qed.
+
+Lemma processed_map_insert `{Countable K} {A}
+    (keys : list K) i key (m : gmap K A) v :
+  NoDup keys →
+  (0 ≤ i)%Z →
+  keys !! Z.to_nat i = Some key →
+  m !! key = Some v →
+  processed_map keys (i + 1) m = <[key:=v]> (processed_map keys i m).
+Proof.
+  intros Hnodup Hi_nonneg Hkey_lookup Hm_lookup.
+  apply map_eq. intros key'.
+  destruct (decide (key' = key)) as [->|Hne].
+  - rewrite lookup_insert_eq /processed_map.
+    apply map_lookup_filter_Some_2; [done|].
+    simpl.
+    replace (Z.to_nat (i + 1)) with (S (Z.to_nat i)) by lia.
+    rewrite (take_S_r _ _ _ Hkey_lookup).
+    rewrite elem_of_list_to_set elem_of_app /=. right. Timeout 10 set_solver.
+  - replace (<[key:=v]> (processed_map keys i m) !! key') with
+      (processed_map keys i m !! key').
+    2:{ symmetry. apply lookup_insert_ne.
+        intro Heq. apply Hne. symmetry. exact Heq. }
+    assert (Hin_iff : key' ∈ list_to_set (C:=gset K)
+        (take (Z.to_nat (i + 1)) keys) ↔
+      key' ∈ list_to_set (C:=gset K) (take (Z.to_nat i) keys)).
+    { replace (Z.to_nat (i + 1)) with (S (Z.to_nat i)) by lia.
+      rewrite (take_S_r _ _ _ Hkey_lookup).
+      rewrite !elem_of_list_to_set elem_of_app /= elem_of_cons elem_of_nil.
+      split; intros Hin.
+      - destruct Hin as [Hin|Hin]; [done|].
+        destruct Hin as [Heq|[]]. subst. contradiction.
+      - left. done. }
+    destruct (m !! key') as [v'|] eqn:Hm_lookup'.
+    + destruct (decide (key' ∈ list_to_set (C:=gset K)
+        (take (Z.to_nat i) keys))) as [Hin|Hnot].
+      * rewrite /processed_map.
+        transitivity (Some v').
+        -- apply map_lookup_filter_Some_2; [done|].
+           simpl. apply Hin_iff. done.
+        -- symmetry. apply map_lookup_filter_Some_2; [done|done].
+      * rewrite /processed_map.
+        transitivity (@None A).
+        -- apply map_lookup_filter_None_2. right.
+           intros x Hx Hin_succ. simpl in Hin_succ.
+           apply Hnot. apply Hin_iff. done.
+        -- symmetry. apply map_lookup_filter_None_2. right.
+           intros x Hx Hin_old. done.
+    + rewrite /processed_map.
+      transitivity (@None A).
+      * apply map_lookup_filter_None_2. left. done.
+      * symmetry. apply map_lookup_filter_None_2. left. done.
+Qed.
+
+Lemma processed_map_all `{Countable K} {A} (keys : list K) (m : gmap K A) :
+  list_to_set keys = dom m →
+  length keys = size m →
+  processed_map keys (Z.of_nat (size m)) m = m.
+Proof.
+  intros Hdom Hlen. apply map_eq. intros key.
+  destruct (m !! key) as [v|] eqn:Hlookup.
+  - rewrite /processed_map. apply map_lookup_filter_Some_2; [done|].
+    simpl. rewrite Nat2Z.id. replace (size m) with (length keys) by done.
+    replace (take (length keys) keys) with keys
+      by (symmetry; apply take_ge; lia).
+    rewrite Hdom elem_of_dom. eexists. exact Hlookup.
+  - rewrite /processed_map. apply map_lookup_filter_None_2. left. done.
+Qed.
+
+Definition obj_list_match (kind namespace : go_string) (kv : KKey.t * KObjectV.t) : Prop :=
+  kv.1.(KKey.Kind') = kind ∧
+  v1.namespace_matches #namespace #(kv.1.(KKey.Namespace')).
+
+Lemma KObjectV_valid_valid_old :
+  ∀ obj, KObjectV.valid obj → KObjectV.valid_old obj.
+Proof.
+  intros [pod|rs] Hvalid.
+  - destruct pod as [tm meta spec status].
+    rewrite /KObjectV.valid /KObjectV.valid_old /PodV.valid
+      /ObjectSpecV.valid /ObjectStatusV.valid /= in Hvalid |- *.
+    destruct Hvalid as (_ & _ & Hmeta & Hspec & Hstatus).
+    split; [exact Hmeta|]. split; [exact Hspec|exact Hstatus].
+  - destruct rs as [tm meta spec status].
+    rewrite /KObjectV.valid /KObjectV.valid_old /ReplicaSetV.valid
+      /ObjectSpecV.valid /ObjectStatusV.valid /= in Hvalid |- *.
+    destruct Hvalid as (_ & _ & Hmeta & Hspec & Hstatus).
+    split; [exact Hmeta|]. split; [exact Hspec|exact Hstatus].
+Qed.
+
+Lemma filtered_processed_map_insert_true kind namespace keys i key abs_state obj :
+  NoDup keys →
+  (0 ≤ i)%Z →
+  keys !! Z.to_nat i = Some key →
+  abs_state !! key = Some obj →
+  obj_list_match kind namespace (key, obj) →
+  filter (obj_list_match kind namespace) (processed_map keys (i + 1) abs_state) =
+    <[key:=obj]> (filter (obj_list_match kind namespace) (processed_map keys i abs_state)).
+Proof.
+  intros Hnodup Hi Hkey_lookup Hobj_lookup Hmatch.
+  rewrite (processed_map_insert keys i key abs_state obj Hnodup Hi Hkey_lookup Hobj_lookup).
+  apply map_filter_insert_True. exact Hmatch.
+Qed.
+
+Lemma filtered_processed_map_insert_false kind namespace keys i key abs_state obj :
+  NoDup keys →
+  (0 ≤ i)%Z →
+  keys !! Z.to_nat i = Some key →
+  abs_state !! key = Some obj →
+  ¬ obj_list_match kind namespace (key, obj) →
+  filter (obj_list_match kind namespace) (processed_map keys (i + 1) abs_state) =
+    filter (obj_list_match kind namespace) (processed_map keys i abs_state).
+Proof.
+  intros Hnodup Hi Hkey_lookup Hobj_lookup Hnot_match.
+  rewrite (processed_map_insert keys i key abs_state obj Hnodup Hi Hkey_lookup Hobj_lookup).
+  apply map_filter_insert_not'.
+  - exact Hnot_match.
+  - intros y Hy. rewrite (processed_map_lookup_not_current keys i key abs_state Hnodup Hkey_lookup Hi) in Hy. done.
+Qed.
+
+Lemma filtered_map_values_valid kind namespace
+    (abs_state : gmap KKey.t KObjectV.t) (used_uid : gset types.UID.t) :
+  (∀ k obj, abs_state !! k = Some obj →
+    k = KObjectV.key obj ∧ KObjectV.valid obj ∧
+    (KObjectV.objectmeta obj).(ObjectMetaV.UID') ∈ used_uid ∧
+    no_speculative_parent_reference (KObjectV.objectmeta obj) used_uid ∧
+    map_Forall (λ k' obj',
+      (KObjectV.objectmeta obj).(ObjectMetaV.UID') =
+        (KObjectV.objectmeta obj').(ObjectMetaV.UID') → k = k') abs_state) →
+  Forall KObjectV.valid
+    (map_to_list (filter (obj_list_match kind namespace) abs_state)).*2.
+Proof.
+  intros Hvalid.
+  rewrite Forall_forall.
+  intros obj Hobj_in.
+  rewrite <- list_elem_of_In in Hobj_in.
+  apply list_elem_of_fmap_1 in Hobj_in as [[k obj'] [Hobj_eq Hkv_in]].
+  simpl in Hobj_eq. subst obj'.
+  apply elem_of_map_to_list in Hkv_in.
+  apply map_lookup_filter_Some in Hkv_in as [Hlookup _].
+  exact (proj1 (proj2 (Hvalid k obj Hlookup))).
+Qed.
+
+Lemma filtered_map_values_valid_old kind namespace
+    (abs_state : gmap KKey.t KObjectV.t) (used_uid : gset types.UID.t) :
+  (∀ k obj, abs_state !! k = Some obj →
+    k = KObjectV.key obj ∧ KObjectV.valid obj ∧
+    (KObjectV.objectmeta obj).(ObjectMetaV.UID') ∈ used_uid ∧
+    no_speculative_parent_reference (KObjectV.objectmeta obj) used_uid ∧
+    map_Forall (λ k' obj',
+      (KObjectV.objectmeta obj).(ObjectMetaV.UID') =
+        (KObjectV.objectmeta obj').(ObjectMetaV.UID') → k = k') abs_state) →
+  Forall KObjectV.valid_old
+    (map_to_list (filter (obj_list_match kind namespace) abs_state)).*2.
+Proof.
+  intros Hvalid.
+  eapply Forall_impl.
+  - intros obj. apply KObjectV_valid_valid_old.
+  - exact (filtered_map_values_valid kind namespace abs_state used_uid Hvalid).
+Qed.
+
+Lemma filtered_map_values_key_eq kind namespace
+    (abs_state : gmap KKey.t KObjectV.t) (used_uid : gset types.UID.t) :
+  (∀ k obj, abs_state !! k = Some obj →
+    k = KObjectV.key obj ∧ KObjectV.valid obj ∧
+    (KObjectV.objectmeta obj).(ObjectMetaV.UID') ∈ used_uid ∧
+    no_speculative_parent_reference (KObjectV.objectmeta obj) used_uid ∧
+    map_Forall (λ k' obj',
+      (KObjectV.objectmeta obj).(ObjectMetaV.UID') =
+        (KObjectV.objectmeta obj').(ObjectMetaV.UID') → k = k') abs_state) →
+  KObjectV.key <$> (map_to_list (filter (obj_list_match kind namespace) abs_state)).*2 =
+    (map_to_list (filter (obj_list_match kind namespace) abs_state)).*1.
+Proof.
+  intros Hvalid.
+  apply list_eq. intros n.
+  rewrite list_lookup_fmap.
+  destruct ((map_to_list (filter (obj_list_match kind namespace) abs_state)).*2 !! n)
+    as [obj|] eqn:Hobj_lookup.
+  - apply list_lookup_fmap_Some_1 in Hobj_lookup as [[k obj'] [Hobj_eq Hkv_lookup]].
+    simpl in Hobj_eq. subst obj'.
+    rewrite list_lookup_fmap Hkv_lookup /=.
+    apply list_elem_of_lookup_2 in Hkv_lookup.
+    apply elem_of_map_to_list in Hkv_lookup.
+    apply map_lookup_filter_Some in Hkv_lookup as [Hlookup _].
+    rewrite (proj1 (Hvalid k obj Hlookup)). done.
+  - destruct ((map_to_list (filter (obj_list_match kind namespace) abs_state)).*1 !! n)
+      as [k|] eqn:Hkey_lookup; [|done].
+    apply list_lookup_fmap_Some_1 in Hkey_lookup as [[k' obj'] [Hkey_eq Hkv_lookup]].
+    simpl in Hkey_eq. subst k'.
+    rewrite list_lookup_fmap Hkv_lookup /= in Hobj_lookup. done.
+Qed.
+
+Lemma filtered_map_values_nodup kind namespace
+    (abs_state : gmap KKey.t KObjectV.t) (used_uid : gset types.UID.t) :
+  (∀ k obj, abs_state !! k = Some obj →
+    k = KObjectV.key obj ∧ KObjectV.valid obj ∧
+    (KObjectV.objectmeta obj).(ObjectMetaV.UID') ∈ used_uid ∧
+    no_speculative_parent_reference (KObjectV.objectmeta obj) used_uid ∧
+    map_Forall (λ k' obj',
+      (KObjectV.objectmeta obj).(ObjectMetaV.UID') =
+        (KObjectV.objectmeta obj').(ObjectMetaV.UID') → k = k') abs_state) →
+  NoDup (KObjectV.key <$> (map_to_list (filter (obj_list_match kind namespace) abs_state)).*2).
+Proof.
+  intros Hvalid.
+  rewrite (filtered_map_values_key_eq kind namespace abs_state used_uid Hvalid).
+  apply NoDup_fst_map_to_list.
 Qed.
 
 Lemma wp_State__objListLocked γ l (kind namespace : go_string) phys_state_l phys_state abs_state used_uid :
@@ -47,7 +294,207 @@ Lemma wp_State__objListLocked γ l (kind namespace : go_string) phys_state_l phy
         end)
   }}}.
 Proof.
-Admitted.
+  wp_start as "H".
+  iNamed "H".
+  iPoseProof (kview.own_auth_valid_forall with "Hown_abs") as "%Habs_valid".
+  wp_auto.
+  iPoseProof (own_slice_nil (V:=interface.t)) as "Hslice_nil".
+  iPoseProof (own_slice_cap_nil (V:=interface.t)) as "Hcap_nil".
+  wp_apply (wp_map_for_range_return_func (key_type:=apimodel.KKey)
+    (λ (keys : list KKey.t) i,
+      ∃ (last_val : interface.t) (last_key : KKey.t)
+        (items_sl : slice.t) (interfaces : list interface.t_ok)
+        (objs : list KObjectV.t),
+        "val" ∷ val_ptr ↦ last_val ∗
+        "key" ∷ key_ptr ↦ last_key ∗
+        "items" ∷ items_ptr ↦ items_sl ∗
+        "kind" ∷ kind_ptr ↦ kind ∗
+        "namespace" ∷ namespace_ptr ↦ namespace ∗
+        "Hitems" ∷ items_sl ↦* (interface.ok <$> interfaces) ∗
+        "Hitems_cap" ∷ own_slice_cap interface.t items_sl (DfracOwn 1) ∗
+        "Hout" ∷ ([∗ list] i; obj ∈ interfaces; objs, KObjectV.deepown_i i obj 1) ∗
+        "Hphys_abs_rep" ∷ ([∗ map] i; obj ∈ phys_state; abs_state,
+          match i with
+          | interface.ok i_ok => KObjectV.deepown_i i_ok obj 1
+          | interface.nil => False%I
+          end) ∗
+        "%Hperm" ∷ ⌜ objs ≡ₚ
+          (map_to_list (filter (obj_list_match kind namespace)
+            (processed_map keys i abs_state))).*2 ⌝)%I
+    with "Hown_phys").
+  { done. }
+  iIntros (keys) "%Hkeys".
+  iSplitL "val key items kind namespace Hslice_nil Hcap_nil Hphys_abs_rep".
+  { iExists interface.nil, (zero_val KKey.t), slice.nil, [], [].
+    iFrame. rewrite big_sepL2_nil.
+    rewrite processed_map_empty map_filter_empty map_to_list_empty.
+    iFrame "Hslice_nil Hcap_nil". done. }
+  iSplitL "".
+  { iModIntro. iIntros (i key phys_obj) "%Hiter Hloop".
+    destruct Hkeys as [Hkeys_dom [Hkeys_len Hkeys_nodup]].
+    destruct Hiter as [Hi_bounds [Hkey_lookup Hphys_lookup]].
+    destruct Hi_bounds as [Hi_nonneg Hi_upper].
+    iDestruct "Hloop" as (last_val last_key items_sl interfaces objs)
+      "(val & key & items & kind & namespace & Hitems & Hitems_cap & Hout & Hphys_abs_rep & %Hperm)".
+    iDestruct (big_sepM2_dom with "Hphys_abs_rep") as %Hdom_eq.
+    assert (∃ obj, abs_state !! key = Some obj) as [obj Habs_lookup].
+    { apply elem_of_dom. rewrite -Hdom_eq. apply elem_of_dom. eexists. done. }
+    iDestruct (big_sepM2_lookup_acc _ _ _ key phys_obj obj
+      Hphys_lookup Habs_lookup with "Hphys_abs_rep") as "[Hdeepown_i Hphys_abs_rep_close]".
+    destruct phys_obj as [i_ok|].
+    2:{ simpl. iDestruct "Hdeepown_i" as %[]. }
+    wp_pures.
+    simpl subst'.
+    wp_auto.
+    destruct (bool_decide (kind = key.(KKey.Kind'))) eqn:Hkind_dec; wp_auto.
+    - destruct (bool_decide (namespace = ""%go)) eqn:Hnamespace_all; wp_auto.
+      + assert (obj_list_match kind namespace (key, obj)) as Hmatch.
+        { split.
+          - apply bool_decide_eq_true in Hkind_dec. done.
+          - unfold v1.namespace_matches.
+            apply bool_decide_eq_true in Hnamespace_all. left. subst. done. }
+        wp_apply (wp_deepCopy with "[$Hdeepown_i]").
+        iIntros (i_copy) "[Hdeepown_copy Hdeepown_i]". wp_auto.
+        wp_apply (wp_slice_literal (V:=interface.t) (t:=go.InterfaceType [])).
+        iSplitR; first done.
+        iIntros (sl_one) "[Hsl_one _]". wp_auto.
+        wp_apply (wp_slice_append with "[$Hitems $Hitems_cap $Hsl_one]").
+        iIntros (items_sl') "(Hitems & Hitems_cap & Hsl_one)". wp_auto.
+        assert (Hsingle :
+          <[sint.nat (W64 0):=interface.ok i_copy]> [interface.nil] =
+          [interface.ok i_copy]).
+        { replace (sint.nat (W64 0)) with 0%nat by word. done. }
+        iEval (rewrite Hsingle) in "Hitems".
+        iDestruct ("Hphys_abs_rep_close" with "Hdeepown_i") as "Hphys_abs_rep".
+        iRight. iSplit; [done|].
+        iExists (interface.ok i_ok), key, items_sl', (interfaces ++ [i_copy]), (objs ++ [obj]).
+        rewrite fmap_app /=.
+        iFrame "val key items kind namespace Hitems Hitems_cap Hphys_abs_rep".
+        iSplitL "Hout Hdeepown_copy".
+        { iApply (big_sepL2_app with "[$Hout]"). iFrame. done. }
+        iPureIntro.
+        assert (Hfiltered_insert :
+          filter (obj_list_match kind namespace) (processed_map keys (i + 1) abs_state) =
+            <[key:=obj]> (filter (obj_list_match kind namespace) (processed_map keys i abs_state))).
+        { apply filtered_processed_map_insert_true; done. }
+        rewrite Hfiltered_insert.
+        assert (Hfiltered_old_lookup :
+          filter (obj_list_match kind namespace) (processed_map keys i abs_state) !! key = None).
+        { apply map_lookup_filter_None_2. left.
+          apply processed_map_lookup_not_current; done. }
+        pose proof (map_to_list_insert
+          (filter (obj_list_match kind namespace) (processed_map keys i abs_state))
+          key obj Hfiltered_old_lookup) as Hinsert_perm.
+        eapply Permutation_trans.
+        * apply Permutation_app; [exact Hperm|done].
+        * etrans.
+          -- symmetry. apply Permutation_middle.
+          -- rewrite app_nil_r.
+             change (((key, obj) :: map_to_list
+                (filter (obj_list_match kind namespace) (processed_map keys i abs_state))).*2
+              ≡ₚ (map_to_list
+                (<[key:=obj]> (filter (obj_list_match kind namespace)
+                  (processed_map keys i abs_state)))).*2).
+             symmetry. apply Permutation_map. exact Hinsert_perm.
+      + destruct (bool_decide (namespace = key.(KKey.Namespace'))) eqn:Hnamespace_eq; wp_auto.
+        * assert (obj_list_match kind namespace (key, obj)) as Hmatch.
+          { split.
+            - apply bool_decide_eq_true in Hkind_dec. done.
+            - unfold v1.namespace_matches.
+              apply bool_decide_eq_true in Hnamespace_eq. right. subst. done. }
+          wp_apply (wp_deepCopy with "[$Hdeepown_i]").
+          iIntros (i_copy) "[Hdeepown_copy Hdeepown_i]". wp_auto.
+          wp_apply (wp_slice_literal (V:=interface.t) (t:=go.InterfaceType [])).
+          iSplitR; first done.
+          iIntros (sl_one) "[Hsl_one _]". wp_auto.
+          wp_apply (wp_slice_append with "[$Hitems $Hitems_cap $Hsl_one]").
+          iIntros (items_sl') "(Hitems & Hitems_cap & Hsl_one)". wp_auto.
+          assert (Hsingle :
+            <[sint.nat (W64 0):=interface.ok i_copy]> [interface.nil] =
+            [interface.ok i_copy]).
+          { replace (sint.nat (W64 0)) with 0%nat by word. done. }
+          iEval (rewrite Hsingle) in "Hitems".
+          iDestruct ("Hphys_abs_rep_close" with "Hdeepown_i") as "Hphys_abs_rep".
+          iRight. iSplit; [done|].
+          iExists (interface.ok i_ok), key, items_sl', (interfaces ++ [i_copy]), (objs ++ [obj]).
+          rewrite fmap_app /=.
+          iFrame "val key items kind namespace Hitems Hitems_cap Hphys_abs_rep".
+          iSplitL "Hout Hdeepown_copy".
+          { iApply (big_sepL2_app with "[$Hout]"). iFrame. done. }
+          iPureIntro.
+          assert (Hfiltered_insert :
+            filter (obj_list_match kind namespace) (processed_map keys (i + 1) abs_state) =
+              <[key:=obj]> (filter (obj_list_match kind namespace) (processed_map keys i abs_state))).
+          { apply filtered_processed_map_insert_true; done. }
+          rewrite Hfiltered_insert.
+          assert (Hfiltered_old_lookup :
+            filter (obj_list_match kind namespace) (processed_map keys i abs_state) !! key = None).
+          { apply map_lookup_filter_None_2. left.
+            apply processed_map_lookup_not_current; done. }
+          pose proof (map_to_list_insert
+            (filter (obj_list_match kind namespace) (processed_map keys i abs_state))
+            key obj Hfiltered_old_lookup) as Hinsert_perm.
+          eapply Permutation_trans.
+          -- apply Permutation_app; [exact Hperm|done].
+          -- etrans.
+             ++ symmetry. apply Permutation_middle.
+             ++ rewrite app_nil_r.
+                change (((key, obj) :: map_to_list
+                  (filter (obj_list_match kind namespace) (processed_map keys i abs_state))).*2
+                ≡ₚ (map_to_list
+                  (<[key:=obj]> (filter (obj_list_match kind namespace)
+                    (processed_map keys i abs_state)))).*2).
+                symmetry. apply Permutation_map. exact Hinsert_perm.
+        * assert (¬ obj_list_match kind namespace (key, obj)) as Hnot_match.
+          { intros [_ Hns_match].
+            unfold v1.namespace_matches in Hns_match.
+            destruct Hns_match as [Hall'|Hns'].
+            - apply bool_decide_eq_false in Hnamespace_all. apply Hnamespace_all.
+              apply go.into_val_inj. rewrite Hall'. done.
+            - apply bool_decide_eq_false in Hnamespace_eq. apply Hnamespace_eq.
+              apply go.into_val_inj. exact Hns'. }
+          iDestruct ("Hphys_abs_rep_close" with "Hdeepown_i") as "Hphys_abs_rep".
+          iRight. iSplit; [done|].
+          iExists (interface.ok i_ok), key, items_sl, interfaces, objs.
+          iFrame. iPureIntro.
+          rewrite (filtered_processed_map_insert_false kind namespace keys i key abs_state obj
+            Hkeys_nodup Hi_nonneg Hkey_lookup Habs_lookup Hnot_match). done.
+    - assert (¬ obj_list_match kind namespace (key, obj)) as Hnot_match.
+      { intros [Hkind _].
+        apply bool_decide_eq_false in Hkind_dec. done. }
+      iDestruct ("Hphys_abs_rep_close" with "Hdeepown_i") as "Hphys_abs_rep".
+      iRight. iSplit; [done|].
+      iExists (interface.ok i_ok), key, items_sl, interfaces, objs.
+      iFrame. iPureIntro.
+      rewrite (filtered_processed_map_insert_false kind namespace keys i key abs_state obj
+        Hkeys_nodup Hi_nonneg Hkey_lookup Habs_lookup Hnot_match). done. }
+  iIntros "Hown_phys Hloop".
+  iDestruct "Hloop" as (last_val last_key items_sl interfaces objs)
+    "(val & key & items & kind & namespace & Hitems & Hitems_cap & Hout & Hphys_abs_rep & %Hperm)".
+  destruct Hkeys as [Hkeys_dom [Hkeys_len Hkeys_nodup]].
+  iDestruct (big_sepM2_dom with "Hphys_abs_rep") as %Hdom_eq.
+  assert (Hkeys_dom_abs : list_to_set keys = dom abs_state).
+  { rewrite Hkeys_dom Hdom_eq. done. }
+  assert (Hkeys_len_abs : length keys = size abs_state).
+  { rewrite Hkeys_len -(size_dom phys_state) Hdom_eq size_dom. done. }
+  assert (Hsize_eq : size phys_state = size abs_state).
+  { rewrite -(size_dom phys_state) Hdom_eq size_dom. done. }
+  rewrite Hsize_eq in Hperm.
+  rewrite (processed_map_all keys abs_state Hkeys_dom_abs Hkeys_len_abs) in Hperm.
+  wp_auto.
+  iApply ("HΦ" $! items_sl interfaces objs). iFrame.
+  iPureIntro. split_and!.
+  - exact Hperm.
+  - eapply Permutation_Forall; [symmetry; exact Hperm|].
+    exact (filtered_map_values_valid kind namespace abs_state used_uid Habs_valid).
+  - eapply Permutation_Forall; [symmetry; exact Hperm|].
+    exact (filtered_map_values_valid_old kind namespace abs_state used_uid Habs_valid).
+  - rewrite (list_fmap_map KObjectV.key objs).
+    rewrite (Permutation_map KObjectV.key Hperm).
+    rewrite -(list_fmap_map KObjectV.key
+      (map_to_list (filter (obj_list_match kind namespace) abs_state)).*2).
+    exact (filtered_map_values_nodup kind namespace abs_state used_uid Habs_valid).
+Qed.
 
 Lemma wp_State__objListLocked_Pod γ l (namespace : go_string) phys_state_l phys_state abs_state used_uid :
   {{{ is_pkg_init apimodel ∗
